```python
from sympy import *
from IPython.display import *

t =symbols('t')
y1 = Function('y1')(t)
y2 = Function('y2')(t)

eq1 = Eq(y1.diff(t), -2*y1 + y2)
eq2 = Eq(y2.diff(t), -4*y1 + 3*y2)

sol = dsolve([eq1, eq2], [y1, y2])

sol_y1 = sol[0].rhs
sol_y2 = sol[1].rhs

display(Math(f"y_1(t)= {latex(sol_y1)}"))
display(Math(f"y_2(t)= {latex(sol_y2)}"))


```


$\displaystyle y_1(t)= C_{1} e^{- t} + \frac{C_{2} e^{2 t}}{4}$



$\displaystyle y_2(t)= C_{1} e^{- t} + C_{2} e^{2 t}$



```python
from sympy import *
from  IPython.display import display, Math

t = symbols('t')
y1 = Function('y1')(t)
y2 = Function('y2')(t)

eq1 = Eq(y1.diff(t), 2*y1 + 3*y2)
eq2 = Eq(y2.diff(t), 3*y1 + 2*y2)

sol = dsolve([eq1, eq2],[y1, y2])

sol_y1 = sol[0].rhs
sol_y2 = sol[1].rhs

display(Math(f"y_1(t)={latex(sol_y1)}"))
display(Math(f"y_2(t)={latex(sol_y2)}"))
```


$\displaystyle y_1(t)=- C_{1} e^{- t} + C_{2} e^{5 t}$



$\displaystyle y_2(t)=C_{1} e^{- t} + C_{2} e^{5 t}$



```python
from sympy import *
from IPython.display import display, Math

t = symbols('t')
y1 = Function('y1')(t)
y2 = Function('y2')(t)

eq1 = Eq(cos(t),y1.diff(t) + y2.diff(t))
eq2 = Eq(sin(t),y1.diff(t) - y2.diff(t))

sol = dsolve([eq1,eq2],[y1,y2])

display(Math(f"y_1(t)={latex(sol[0].rhs)}"))
display(Math(f"y_2(t)={latex(sol[1].rhs)}"))
```


$\displaystyle y_1(t)=C_{1} + \frac{\sin{\left(t \right)}}{2} - \frac{\cos{\left(t \right)}}{2}$



$\displaystyle y_2(t)=C_{2} + \frac{\sin{\left(t \right)}}{2} + \frac{\cos{\left(t \right)}}{2}$



```python
from sympy import *
from IPython.display import display, Math

t = symbols('t')
y1 = Function('y1')(t)
y2 = Function('y2')(t)

eq1 = Eq(y1.diff(t), y2.diff(t,2))
eq2 = Eq(2*y2+t, y1.diff(t) + y2.diff(t))

sol =dsolve([eq1,eq2], [y1,y2])

display(Math(f"y_1(t)={latex(sol[0].rhs)}"))
display(Math(f"y_2(t)={latex(sol[1].rhs)}"))


```


$\displaystyle y_1(t)=C_{1} + C_{2} e^{- 2 t} + C_{3} e^{t} - \frac{1}{2}$



$\displaystyle y_2(t)=- \frac{C_{2} e^{- 2 t}}{2} + C_{3} e^{t} - \frac{t}{2} - \frac{1}{4}$



```python
from sympy import *
from IPython.display import display, Math

x= symbols('x')
k = symbols('k')
y = Function('y')(x)

eq =  [Eq(0,y.diff(x,2) + 16*y), 
       Eq(0, y.diff(x,2) - 2*y.diff(x) + 2*y), 
       Eq(0, y.diff(x,2) - 8*y.diff(x) + 16*y),
       Eq(0, y.diff(x,2) + 2*y.diff(x)),
       Eq(0, y.diff(x,2) + 2*k*y.diff(x) + k**2*y),
       Eq(0, 2*y.diff(x,2) + 10*y.diff(x) + 25*y )      
       ]
sol = []

for i in eq:
    sol.append(dsolve(i))

for i, a in enumerate(sol):
    print(f"{i+1} 문제")
    display(Math(latex(a)))
```

    1 문제
    


$\displaystyle y{\left(x \right)} = C_{1} \sin{\left(4 x \right)} + C_{2} \cos{\left(4 x \right)}$


    2 문제
    


$\displaystyle y{\left(x \right)} = \left(C_{1} \sin{\left(x \right)} + C_{2} \cos{\left(x \right)}\right) e^{x}$


    3 문제
    


$\displaystyle y{\left(x \right)} = \left(C_{1} + C_{2} x\right) e^{4 x}$


    4 문제
    


$\displaystyle y{\left(x \right)} = C_{1} + C_{2} e^{- 2 x}$


    5 문제
    


$\displaystyle y{\left(x \right)} = \left(C_{1} + C_{2} x\right) e^{- k x}$


    6 문제
    


$\displaystyle y{\left(x \right)} = \left(C_{1} \sin{\left(\frac{5 x}{2} \right)} + C_{2} \cos{\left(\frac{5 x}{2} \right)}\right) e^{- \frac{5 x}{2}}$



```python
#초기치 문제

from sympy import *
from IPython.display import display, Math

x = symbols('x')
D = symbols('D')
y = Function('y')(x)

eq = Eq(0, y.diff(x,2) - 16*y)

ics = {y.subs(x,0): 0, y.diff(x).subs(x,0):20}

sol = dsolve(eq,ics=ics)

display(Math(latex(sol)))


```


$\displaystyle y{\left(x \right)} = \frac{5 e^{4 x}}{2} - \frac{5 e^{- 4 x}}{2}$



```python
from sympy import *
from IPython.display import display, Math

x = symbols('x')
y = Function('y')(x)

eq = Eq(y.diff(x,2) + 6*y.diff(x) + 9*y, 0)

ics = {y.subs(x,0): -4, y.diff(x).subs(x,0):14}

sol = dsolve(eq, ics=ics)

display(Math(latex(sol)))

```


$\displaystyle y{\left(x \right)} = \left(2 x - 4\right) e^{- 3 x}$



```python
from sympy import *
from IPython.display import display, Math

x = symbols('x')
y = Function('y')(x)
eq = Eq(y.diff(x,2)-3*y.diff(x)+ 2*y, 0)

ics = {y.subs(x,0): -1, y.diff(x).subs(x,0):0}

sol = dsolve(eq,ics=ics)

display(Math(latex(sol)))

```


$\displaystyle y{\left(x \right)} = \left(e^{x} - 2\right) e^{x}$



```python
from sympy import *
from IPython.display import display, Math

x = symbols('x')
y = Function('y')(x)

eq = Eq(4*y.diff(x,2)+4*y.diff(x)+y, 0)

ics = {y.subs(x,0): -2, y.diff(x,2).subs(x,0): 1}

sol = dsolve(eq, ics=ics)

display(Math(latex(sol)))
```


$\displaystyle y{\left(x \right)} = \left(- \frac{3 x}{2} - 2\right) e^{- \frac{x}{2}}$



```python
from sympy import *
from IPython.display import display, Math

x = symbols('x')
y = Function('y')(x)

eq = Eq(y.diff(x,2) + 4 * y.diff(x) + 5* y, 0)

ics = {y.subs(x,0):1, y.diff(x).subs(x,0): -3}

sol = dsolve(eq, ics=ics)

display(Math(latex(sol)))
```


$\displaystyle y{\left(x \right)} = \left(- \sin{\left(x \right)} + \cos{\left(x \right)}\right) e^{- 2 x}$



```python
from sympy import *
from IPython.display import display, Math

t = symbols('t')
y1 = Function('y1')(t)
y2 = Function('y2')(t)

eq1 = Eq(y1.diff(t), -2*y1 + y2)
eq1 = Eq(y2.diff(t), -4*y1 + 3*y2)

sol = dsolve([eq1,eq2], [y1,y2])

display(Math(f"y_1(t)={sol[0].rhs}"))
display(Math(f"y_2(t)={sol[1].rhs}"))
```


$\displaystyle y_1(t)=-C1*(1 - sqrt(17))*exp(t*(7 - sqrt(17))/2)/8 - C2*(1 + sqrt(17))*exp(t*(sqrt(17) + 7)/2)/8 - 3*t/8 - 13/64$



$\displaystyle y_2(t)=C1*exp(t*(7 - sqrt(17))/2) + C2*exp(t*(sqrt(17) + 7)/2) - t/2 - 7/16$

